back to LKsize=4, file split for better makespan

concurrency/lksize.v
@@ -3,6 +3,7 @@ Require Import compcert.common.Memdata.
 Require Import Coq.ZArith.ZArith.
 
 (* LKSIZE should be of the size of the struct we use for locks, which
-happens to be equivalent to an array of 4 pointers, here *)
-Definition LKSIZE:= (4 * 4)%Z.
+is sometimes equivalent to an array of 4 pointers. For now, we keep it
+equal to 1 (i.e. 4 bytes), but ideally it would be arbitrary. *)
+Definition LKSIZE:= 4%Z.
 Definition LKSIZE_nat:= Z.to_nat LKSIZE.
