concurrency/semax_preservation_makelock.v
@@ -1,0 +1,255 @@
+Require Import Coq.Strings.String.
+
+Require Import compcert.lib.Integers.
+Require Import compcert.common.AST.
+Require Import compcert.cfrontend.Clight.
+Require Import compcert.common.Globalenvs.
+Require Import compcert.common.Memory.
+Require Import compcert.common.Memdata.
+Require Import compcert.common.Values.
+
+Require Import msl.Coqlib2.
+Require Import msl.eq_dec.
+Require Import msl.seplog.
+Require Import veric.initial_world.
+Require Import veric.juicy_mem.
+Require Import veric.juicy_mem_lemmas.
+Require Import veric.semax_prog.
+Require Import veric.compcert_rmaps.
+Require Import veric.Clight_new.
+Require Import veric.Clightnew_coop.
+Require Import veric.semax.
+Require Import veric.semax_ext.
+Require Import veric.juicy_extspec.
+Require Import veric.juicy_safety.
+Require Import veric.initial_world.
+Require Import veric.juicy_extspec.
+Require Import veric.tycontext.
+Require Import veric.semax_ext.
+Require Import veric.res_predicates.
+Require Import veric.mem_lessdef.
+Require Import floyd.coqlib3.
+Require Import sepcomp.semantics.
+Require Import sepcomp.step_lemmas.
+Require Import sepcomp.event_semantics.
+Require Import sepcomp.semantics_lemmas.
+Require Import concurrency.coqlib5.
+Require Import concurrency.permjoin.
+Require Import concurrency.semax_conc.
+Require Import concurrency.juicy_machine.
+Require Import concurrency.concurrent_machine.
+Require Import concurrency.scheduler.
+Require Import concurrency.addressFiniteMap.
+Require Import concurrency.permissions.
+Require Import concurrency.JuicyMachineModule.
+Require Import concurrency.age_to.
+Require Import concurrency.sync_preds_defs.
+Require Import concurrency.sync_preds.
+Require Import concurrency.join_lemmas.
+Require Import concurrency.aging_lemmas.
+Require Import concurrency.cl_step_lemmas.
+Require Import concurrency.resource_decay_lemmas.
+Require Import concurrency.resource_decay_join.
+Require Import concurrency.semax_invariant.
+Require Import concurrency.semax_simlemmas.
+Require Import concurrency.sync_preds.
+Require Import concurrency.lksize.
+Require Import concurrency.rmap_locking.
+
+Local Arguments getThreadR : clear implicits.
+Local Arguments getThreadC : clear implicits.
+Local Arguments personal_mem : clear implicits.
+Local Arguments updThread : clear implicits.
+Local Arguments updThreadR : clear implicits.
+Local Arguments updThreadC : clear implicits.
+Local Arguments juicyRestrict : clear implicits.
+
+Set Bullet Behavior "Strict Subproofs".
+
+Open Scope string_scope.
+
+(* to make the proof faster, we avoid unfolding of those definitions *)
+Definition Jspec'_juicy_mem_equiv_def CS ext_link :=
+  ext_spec_stable juicy_mem_equiv (JE_spec _ ( @OK_spec (Concurrent_Espec unit CS ext_link))).
+
+Definition Jspec'_hered_def CS ext_link :=
+   ext_spec_stable age (JE_spec _ ( @OK_spec (Concurrent_Espec unit CS ext_link))).
+
+Lemma preservation_makelock
+  (lockSet_Writable_updLockSet_updThread
+     : forall (m m' : Memory.mem) (i : tid) (tp : thread_pool) (Phi : LocksAndResources.res),
+       mem_compatible_with tp m Phi ->
+       forall (cnti : containsThread tp i) (b : block) (ofs : int) (ophi : option rmap)
+         (ophi' : LocksAndResources.lock_info) (c' : ctl) (phi' : LocksAndResources.res) 
+         (z : int) (pr : mem_compatible tp m),
+       AMap.find (elt:=option rmap) (b, Int.intval ofs) (lset tp) = Some ophi ->
+       Mem.store Mint32 (restrPermMap (mem_compatible_locks_ltwritable pr)) b (Int.intval ofs) (Vint z) = Some m' ->
+       lockSet_Writable (lset (updLockSet (updThread i tp cnti c' phi') (b, Int.intval ofs) ophi')) m') 
+  (mem_cohere'_store : forall m tp m' b ofs i Phi
+    (Hcmpt : mem_compatible tp m),
+    lockRes tp (b, Int.intval ofs) <> None ->
+    Mem.store
+      Mint32 (restrPermMap (mem_compatible_locks_ltwritable Hcmpt))
+      b (Int.intval ofs) (Vint i) = Some m' ->
+    mem_compatible_with tp m Phi (* redundant with Hcmpt, but easier *) ->
+    mem_cohere' m' Phi)
+  (personal_mem_equiv_spec
+     : forall (m m' : Mem.mem') (phi : rmap) (pr : mem_cohere' m phi) (pr' : mem_cohere' m' phi),
+       Mem.nextblock m = Mem.nextblock m' ->
+       (forall loc : address, max_access_at m loc = max_access_at m' loc) ->
+       (forall loc : AV.address, isVAL (phi @ loc) -> contents_at m loc = contents_at m' loc) ->
+       mem_equiv (m_dry (personal_mem m phi pr)) (m_dry (personal_mem m' phi pr')))
+  (CS : compspecs)
+  (ext_link : string -> ident)
+  (ext_link_inj : forall s1 s2, ext_link s1 = ext_link s2 -> s1 = s2)
+  (Jspec' := @OK_spec (Concurrent_Espec unit CS ext_link))
+  (Jspec'_juicy_mem_equiv : Jspec'_juicy_mem_equiv_def CS ext_link)
+  (Jspec'_hered : Jspec'_hered_def CS ext_link)
+  (Gamma : PTree.t funspec)
+  (n : nat)
+  (ge : SEM.G)
+  (m m' : Memory.mem)
+  (i : tid)
+  (sch : list tid)
+  (tp tp' : thread_pool)
+  (INV : state_invariant Jspec' Gamma (S n) (m, ge, (i :: sch, tp)))
+  (Phi : rmap)
+  (compat : mem_compatible_with tp m Phi)
+  (lev : level Phi = S n)
+  (gam : matchfunspec (filter_genv ge) Gamma Phi)
+  (sparse : lock_sparsity (lset tp))
+  (lock_coh : lock_coherence' tp Phi m compat)
+  (safety : threads_safety Jspec' m ge tp Phi compat (S n))
+  (wellformed : threads_wellformed tp)
+  (unique : unique_Krun tp (i :: sch))
+  (Ei cnti : ssrnat.leq (S i) (pos.n (num_threads tp)) = true)
+  (ci : code)
+  (Eci : getThreadC i tp cnti = Kblocked ci)
+  (ev : Events.sync_event)
+  (Hcmpt : mem_compatible tp m)
+  (Htid : ssrnat.leq (S i) (pos.n (num_threads tp)) = true)
+  (HschedN : SCH.schedPeek (i :: sch) = Some i)
+  (Htstep : syncStep ge Htid Hcmpt tp' m' ev)
+  (jmstep : @JuicyMachine.machine_step ge (i :: sch) nil tp m sch nil tp' m')
+  (tp_ := tp' : thread_pool)
+  (m_ := m' : Memory.mem)
+  (El : Logic.True -> level (getThreadR i tp Htid) - 1 = n)
+  (compat_aged : mem_compatible_with (age_tp_to n tp) m (age_to n Phi))
+  (tp'0 tp'' : thread_pool)
+  (jm : juicy_mem)
+  (c : code)
+  (b : block)
+  (ofs : int)
+  (R : pred rmap)
+  (phi' : rmap)
+  (m'0 : Memory.mem)
+  (Hcompatible : mem_compatible tp m)
+  (Hinv : invariant tp)
+  (Hthread : getThreadC i tp Htid = Kblocked c)
+  (Hat_external : at_external SEM.Sem c = Some (MKLOCK, Vptr b ofs :: nil))
+  (* (Hright_juice : m = m_dry jm) *)
+  (Hpersonal_perm : personal_mem m (getThreadR i tp Htid) (thread_mem_compatible Hcompatible Htid) = jm)
+  (Hpersonal_juice : getThreadR i tp Htid = m_phi jm)
+  (Hstore : Mem.store Mint32 (m_dry jm) b (Int.intval ofs) (Vint Int.zero) = Some m')
+  (Hrmap : rmap_makelock (getThreadR i tp cnti) phi' (b, Int.unsigned ofs) R LKSIZE)
+  (Htp' : tp'0 = updThread i tp Htid (Kresume c Vundef) phi')
+  (Htp'' : tp' = age_tp_to (level (m_phi jm) - 1) (updLockSet tp'0 (b, Int.intval ofs) None))
+  (H : tp'' = tp')
+  (H0 : m'0 = m')
+  (H1 : Events.mklock (b, Int.intval ofs) = ev) :
+  (* ============================ *)
+  state_invariant Jspec' Gamma n (m_, ge, (sch, tp_)).
+
+Proof.
+    (* now much easier with rmap_makelock.
+    (* we must define the new Phi *)
+    
+    Definition rmap_makelock phi phi' sh loc R :=
+      (forall x, ~ adr_range loc LKSIZE x -> phi @ x = phi' @ x) /\
+      (forall x, adr_range loc LKSIZE x -> exists val, phi @ x = YES sh pfullshare (VAL val) NoneP) /\
+      (LKspec_ext R fullshare fullshare loc phi').
+    Definition rmap_freelock phi phi' sh loc R :=
+      (forall x, ~ adr_range loc LKSIZE x -> phi @ x = phi' @ x) /\
+      (LKspec_ext R fullshare fullshare loc phi) /\
+      (forall x, adr_range loc LKSIZE x -> exists val, phi' @ x = YES sh pfullshare (VAL val) NoneP).
+    
+    assert (HPhi' : exists Phi', rmap_makelock Phi Phi' sh (b, Int.intval ofs) R). {
+(*      pose (f' :=
+              fun loc =>
+                if adr_range_dec (b, Int.intval ofs) LKSIZE loc then
+                  if eq_dec (Int.intval ofs) (snd loc) then
+                    LK  *)
+      admit.
+    }
+    destruct HPhi' as (Phi' & HPhi').
+    
+    subst m_ tp' tp'0 m'0.
+    pose (tp2 := (updLockSet (updThread i tp Htid (Kresume c Vundef) phi') (b, Int.intval ofs) None)).
+    fold tp2 in H.
+    assert (compat' : mem_compatible_with tp2 m' Phi'). {
+      unfold tp2.
+      (*
+      below, without the modification of the Phi'
+      rewrite <-Hpersonal_juice.
+      rewrite El.
+      constructor.
+      - (* joining to global map: the acquired rmap move from
+            lockset to threads's maps *)
+        pose proof juice_join compat as J.
+        apply join_all_age_to. cleanup. omega.
+        rewrite join_all_joinlist in J |- *.
+        rewrite maps_updlock1.
+        rewrite maps_remLockSet_updThread.
+        rewrite maps_updthread.
+        erewrite (maps_getthread i _ Htid) in J; eauto.
+        clear -J Hct0 Hct Hj_forward Hpersonal_juice lock_coh levphi' Hlock.
+        rewrite maps_getlock1; swap 1 2. {
+          specialize (lock_coh (b, Int.intval ofs)).
+          cleanup.
+          destruct (AMap.find _ _) as [o|]; auto. exfalso.
+          specialize (Hct (Int.intval ofs)).
+          assert_specialize Hct. split. omega. unfold LKSIZE; simpl. omega.
+          destruct Hct as (val & sh'' & E).
+          assert (j : join_sub (getThreadR i tp Htid) Phi) by apply compatible_threadRes_sub, compat.
+          destruct j as (?, j).
+          apply resource_at_join with (loc := (b, Int.intval ofs)) in j.
+          rewrite Hpersonal_juice in j.
+          rewrite E in j.
+          destruct o.
+          - destruct lock_coh as (_ & sh' & R' & lk & _).
+            apply predat2 in lk.
+            unfold predat in *.
+            inv j; breakhyps.
+          - destruct lock_coh as (_ & sh' & R' & lk).
+            apply predat2 in lk.
+            unfold predat in *.
+            inv j; breakhyps.
+        }
+        destruct J as (psi & j1 & j2).
+        exists psi; split; auto.
+        apply resource_at_join2.
+        + rewrite levphi'. rewrite <-Hpersonal_juice. join_level_tac.
+        + join_level_tac.
+        + intros (b', ofs').
+          rewrite Hpersonal_juice in j2.
+          apply resource_at_join with (loc := (b', ofs')) in j2.
+          specialize (Hj_forward (b', ofs')). simpl in Hj_forward.
+          destruct (adr_range_dec (b, Int.intval ofs) 4 (b', ofs')) as [a|a]; swap 1 2.
+          * assert_specialize Hj_forward. 2:congruence.
+            unfold adr_range in *.
+            unfold LKSIZE in *.
+            simpl. cut ( b <> b' \/ ~ (Int.intval ofs <= ofs' < Int.intval ofs + 4)%Z). admit. (* wtf machine *)
+            tauto.
+          * unfold adr_range in *.
+            destruct a as [<- a].
+            specialize (Hct ofs'). autospec Hct.
+            destruct Hct as (val & sh' & E).
+            rewrite E in j2.
+            destruct (eq_dec ofs' (Int.intval ofs)) as [e|e].
+            -- subst ofs'.
+               rewrite Hlock.
+               inv j2.
+               ++ (* NOT THE SAME PHI *)
+                 admit.
+       *) *)
+Admitted.
